some thoughts in

Coq/MutatorCount.v
@@ -8,12 +8,19 @@ Set Implicit Arguments.
 Unset Strict Implicit.
 Unset Printing Implicit Defensive. 
 
+Lemma find_first {A: eqType} (l : seq A) f : has f l ->
+  exists e l1 l2, [/\ l = l1 ++ e :: l2, f e & ~~ has f l1].
+Proof.
+elim:l=>//= e l Hi; case X : (f e)=>/=.
+- by move=> _; exists e, [::], l; rewrite cat0s.
+case/Hi=>e'[l1][l2][E1]H1 H2.
+by exists e', (e:: l1), l2; rewrite E1/= X H2/= H1. 
+Qed.
+
 Section MutatorCount.
 
 Variable e0 : LogEntry.
 (* Initial graph an heap *)
-Variables (h0 : heap) (g0: graph h0).
-
 
 (* A number of references from behind of wavefront to o, obtained as a
    result of mutation. *)
@@ -41,33 +48,111 @@ Definition M_minus l o f n : nat := size
 
 (* A T-entry e records exactly the new value of a MA-entry *)
 
-Definition matchingT ema := fun e =>
+Definition matchingTFull ema := fun e =>
    [&& kind e == T, fld e == fld ema,
        source e == source ema & new e == new ema].
 
+Definition matchingT ema := fun e =>
+   [&& kind e == T, fld e == fld ema & source e == source ema].
 
-Lemma mut_count l h (g : graph h) et ema l1 l2 l3 :
+
+(* Lemma mut_count_inv h0 (g0 : graph h0) l h (g : graph h) et l2 : *)
+(*    executeLog g0 l = Some {| hp := h; gp := g |} -> *)
+(*    l = et :: l2 -> kind et == T -> *)
+(*    ~~ has (matchingTFull ema) l -> *)
+(*    M_minus l (source et) (fld et) (new et) <= *)
+(*    M_plus l (source et) (fld et) (new et). *)
+(* Proof.  *)
+(* 
+
+A general invariant for the mutator count for a specific object-field
+(o, f) should state that for any triple (o, f, n), if 
+
+- l = et :: l2, and et traces (o, f)
+- there is no entry in l that traces "n" of (o, f),
+
+Then M+(o, f, n) >= M-(o, f, n). 
+
+The tricky part of the proof is dealing with decrements of the mutator
+count. In this case, we should show that previously the inequality
+was, actually, strict, as there should've been an immeditely preceding
+entry, assigning this field. The last fact should be a separate lemma. 
+
+Also, we need to prove some distributivity facts of M+ and M- over
+logs.
+ 
+
+*)
+
+
+
+
+
+Lemma mut_count_trimmed h0 (g0 : graph h0) l h (g : graph h) et ema l2 :
    executeLog g0 l = Some {| hp := h; gp := g |} ->
-   l = l1 ++ et :: l2 ++ ema :: l3 -> kind et == T ->
+   l = (et :: rcons l2 ema) -> kind et == T ->
    matchingMA (source et) (fld et) ema ->
    source et # fld et @ g = new ema ->
-   ~~ has (matchingT ema) l ->
+   ~~ has (matchingTFull ema) l ->
+   M_minus l (source ema) (fld ema) (new ema) <
+   M_plus l (source ema) (fld ema) (new ema).
+Proof. 
+(* 
+
+The proof of this fact goes by induction on l2, however, the inductive
+invariant is somewhat tricky. In particular, we should ensure that for
+each decrement of the mutator count, there should be a preceding
+entry, which increases it. So, see a more general previous statement.
+
+
+
+ *)
+Admitted.
+
+
+
+Lemma mut_count h0 (g0 : graph h0) l h (g : graph h) et ema l1 l2 l3 :
+   executeLog g0 l = Some {| hp := h; gp := g |} ->
+   l = l1 ++ (et :: rcons l2 ema) ++ l3 -> kind et == T ->
+   matchingMA (source et) (fld et) ema ->
+   source et # fld et @ g = new ema ->
+   ~~ has (matchingTFull ema) l ->
+   ~~ has (matchingT ema) l1 ->
    ~~ has (matchingMA (source et) (fld et)) l3 ->
    M_minus l (source ema) (fld ema) (new ema) <
    M_plus l (source ema) (fld ema) (new ema).
-Proof. Admitted. 
+Proof. 
+
+(* 
+
+The proof of this lemma should be reucible to the proof of the
+previous fact, mu_count_clean, which trims the lists l1 and l3,
+because of the following reasons:
+
+   - l1 doesn't have entries that can affect the wavefront wrt. ema's
+     parameters (o, f), so excluding it doesn't change M+ and M-.
+   
+   - l3 doesn't have MA-entries with the same source/field, hence it
+     doesn't affect the values of M+ and M-
+
+   The proofs of these "trimming" lemmas should be explicitly
+   constructed. So, for now see the previous statement
+
+*)
+
+Admitted. 
 
 
 (* The following lemma is the key for the proof of expose_c soundness,
    as it justifies the use of the mutator count as a valid way to expose
    reachable objects. *)
 
-Lemma mut_count_fires l h (g : graph h) et ema l1 l2 l3 :
+Lemma mut_count_fires h0 (g0 : graph h0) l h (g : graph h) et ema l1 l2 l3 :
    executeLog g0 l = Some {| hp := h; gp := g |} ->
    l = l1 ++ et :: l2 ++ ema :: l3 -> kind et == T ->
    matchingMA (source et) (fld et) ema ->
    source et # fld et @ g = new ema ->
-   ~~ has (matchingT ema) l ->
+   ~~ has (matchingTFull ema) l ->
    ~~ has (matchingMA (source et) (fld et)) l3 ->
    (source ema, fld ema, new ema) \in 
        [seq (source pi, fld pi, new pi) | 
@@ -79,7 +164,18 @@ suff X: (M_minus l (source ema) (fld ema) (new ema) <
          M_plus  l (source ema) (fld ema) (new ema)).
 - apply/mapP; exists ema=>//.
   by rewrite mem_filter X E//= mem_cat inE mem_cat inE eqxx -!(orbC true). 
-by apply: (@mut_count l h g et ema l1 l2 l3).
+have X: has (matchingT ema) (l1 ++ [:: et]).
+- rewrite has_cat/= -!(orbC false)/=; apply/orP; right.
+  rewrite /matchingT; case/andP: M=>_/andP[/eqP->]/eqP->. 
+  by rewrite K !eqxx.
+case: (find_first X)=>et'[l1'][l2'][E2]H3 H4.
+rewrite -cat_cons catA -(cat_rcons et) -cats1 E2 -!catA in E.
+rewrite cat_cons -(cat_rcons ema) -cats1 in E.
+rewrite catA cats1 -rcons_cat -(cat_cons et') in E. 
+case/andP: (H3)=>Z/andP[/eqP A2]/eqP A1.
+case/andP: (M)=>_/andP[/eqP B1]/eqP B2.
+rewrite B1 -A1 B2 -A2 in M E1 H2.
+by apply: (@mut_count h0 g0 l h g et' ema l1' (l2' ++ l2) l3)=>//.
 Qed.
 
 
